# Summary
# Related

Prev - [[1.4 Using the Definitions of the Trigonometric Functions]]
Next - [[2.2 Trigonometric Functions of Non-Acute Angles]]
# Content

Right triangle based definitions of Trigonometric Functions (for any acute angle A in standard position).

![[right_triangles.jpg]]
This is where you'll likely use the Soh Cah Toa

You may see questions like
@**Insert question pic here**

@**Insert answer pic here**

>[!note]
>D + E = $90\degree$ which makes D & E *Complimentary Angels*.
>
>As such:
>sinD = cosE
>cosD = sinE
>tanD = cotE
>cotD = tanE
>cscD = secE
>secD = cscD
>
>These above are called *Cofunctions* of on another. Which means that the angles are complimentary and the function values are equal.

>[!note] Cofunction Identities
>For any acute angle A.
>sinA = cos(90-A)
>cosA = sin(90-A)
>tanA = cot(90-A)
>cotA = tan(90-A)
>secA = csc(90-A)
>cscA = sec(90-A)
>
>Same pattern, different function.

>[!faq]- Write each in terms of its cofunction. $\sin9\degree=\cos(90-A)$ & $\cot76\degree=\tan(90-A)$
>$\sin9\degree=\cos(90-A)$
>$\sin9\degree=\cos(90-9)=\cos81\degree$
>$\cot76\degree=\tan(90-A)$
>$\cot76\degree=\tan(90-76)=\tan14\degree$

>[!faq]- Find a solution for the equation. Assume all angles in which an unknown appears are acute angles: $\cos=\sin(\alpha+30\degree)$
>Since $\cos \theta$ and $\sin \theta$ are cofunctions, they are related by identity.
>
>$\cos \theta=\sin(90-\theta)$
>
>Thus, for acute angles, if a function and the cofunction values are equal, the sum of the angles **MUST** be $90\degree$.
>
>$\alpha+\alpha+30\degree=90\degree$
>$2\alpha+30\degree=90\degree$
>$2\alpha=60$
>$\alpha=30\degree$
>
>So the solution for the equation is $30\degree$

If you encounter one worded like this $\cot (\theta-8\degree)=\tan(40+13\degree)$ then just plug it into the function instead and foil.

$\cot(\theta-8)=\cot(90-(40+13))$ becomes $\theta-8=90-40-13$
Which then solves down to $\theta=17\degree$

>[!info] Memorize
>That a right triangle with degrees of both 45 then the sides are 1 and the hypotenuse is $\sqrt{ 2 }$. You may remember this from the [[UnitCircle.png]].

>[!faq]- Find the equation of a line passing through the point (0,4) and making a $45\degree$ with the line.
>Given (0,4) you know that y=4
>And you can work out that $45\degree$ is a *TAN* angle and equates out to 1
>
>So that 1 will be times your X, rather redundant in this case, plus your Y, which is already said to be 4.
>
>Answer: y = x + 4

>[!faq]- Find the equation of a line passing through the point (0,3) and making a $60\degree$ with the line.
>Same as the one above, your Y is already said to be 3.
>Now just find the *TAN* of $60\degree$ which equates out to $\sqrt{ 3 }$
>
>Just plug that in and you get: $y=\sqrt{ 3 }x+3$

>[!faq]- ![[2.1 HW.png]]
>Start by finding the value of **m**
>The length of the hypotenuse is known, therefore, the cosine function will allow the length of **m** to be calculated because the right-triangle-based definition of cosine is $\frac{adjacent}{hypotenuse}$.
>The value of $\cos30\degree$ is $\frac{\sqrt{ 3 }}{2}$
>
>Now just solve with what you have for **m** $\frac{\sqrt{ 3 }}{2}=\frac{a}{21}$
>Multiply 21 by both sides to get **a** by itself: $m=\frac{21\sqrt{ 3 }}{2}$
>
>Since the relationship between the angles is $30\degree-60\degree$ then all you need to do is halve **m** get **g** which is $10\frac{1}{2}$
>
>Once you have **g** you can use the same process on the second triangle and just work from there to fill in all the sides, but use the sine function for $60\degree$ angles because $\sin=\frac{opposite}{hypotenuse}$, which $\sin 60\degree=\frac{\sqrt{ 3 }}{2}$
>
>So $\frac{\sqrt{ 3 }}{2}=\frac{10\frac{1}{2}}{h}$
>First simplify $10\frac{1}{2}$ which is just $10*\frac{1}{2}$ to just 21 making the right side $\frac{21}{2}$.
>$\frac{\sqrt{ 3 }}{2}=\frac{\frac{21}{2}}{c}$ Now multiply both sides by **c**
>$c \frac{\sqrt{ 3 }}{2}=\frac{21}{2}$ Now just multiply both sides by $\frac{\sqrt{ 3 }}{2}$ of course now flipped
>$\frac{21}{2}*\frac{2}{\sqrt{ 3 }}=\frac{42}{2\sqrt{ 3 }}$ then rationalize $\frac{42}{2\sqrt{ 3 }}*\frac{2\sqrt{ 3 }}{2\sqrt{ 3 }}=\frac{84\sqrt{ 3 }}{12}$
>Then just simplify $\frac{84\sqrt{ 3 }}{12}=7\sqrt{ 3 }$
>So, side **h** = $7\sqrt{ 3 }$
>
>Finally, since the relationship with the angles is again $30\degree-60\degree$ you can just use half the **hypotenuse** again to simply get **n**
>$\frac{7\sqrt{ 3 }}{2}$ Which can't be simplified so **n** is simply $\frac{7\sqrt{ 3 }}{2}$



# References

Lesson 2024-02-20