>[!faq]- Find the limit of $\lim_{ x \to 9^+ }\frac{\mid9-x\mid}{9-x}$
>Substitute: $$\frac{\mid 9-(9)\mid}{9-(9)}$$
>Simplify and remember it comes from the right: $$\frac{0}{0}=1=-1$$

>[!faq]- Find the limit of $\lim_{ x \to 0 }\frac{x^2-2x+\sin x}{x}$
>Separate out: $$\frac{x^2}{x}-\frac{2x}{x}+\frac{\sin x}{x}$$
>Simplify: $$x-2+\frac{\sin x}{x}$$
>Substitute: $$(0)-2+\frac{\sin(0)}{0}$$
>Simplify: $$-2+\frac{0}{0}$$
>$$-2+1$$
>$$-1$$

>[!faq]- Find the vertical asymptotes of $f(x)=\frac{x-3}{9x-x^3}$
>Factor out __x__: $$\frac{x-3}{x(9-x^2)}$$
>Separate the binomial: $$\frac{x-3}{x(x-3)(x+3)}$$
>Like terms: $$\frac{1}{x(x+3)}$$
>Take both and set them equal to __0__: $$x=0$$
>$$x+3=0$$
>Find __x__ for both: $$x=0$$
>$$x=-3$$

>[!faq]- Find the vertical asymptotes of $f(x)=\frac{-x^2+16}{x^2+fx+4}$
>Factor out negative: $$\frac{x^2-16}{x^2+5x+4}$$
>Factor numerator: $$\frac{(x-4)(x+4)}{x^2+5x+4}$$
>Factor denominator: $$\frac{(x-4)(x+4)}{(x+1)(x+4)}$$
>Like terms: $$\frac{(x-4)}{(x+1)}$$
>Set equal to __0__ and solve: $$x=4,x=-1$$
>Plug back in and check: $$(4)^2-16=0$$
>__4__ can't work, so that just leaves __-1__ which does.

