# Summary

# Learning Objectives
- Find the [[derivative]] of a composite [[function]] using [[Chain Rule]].
- Find the [[derivative]] of a [[function]] using [[General Power Rule]].
- Simplify the [[derivative]] of a [[function]] using algebra.
- Find the [[derivative]] of a trigonometric [[function]] using [[Chain Rule]].
# Related
Prev - [[2.3 Product and Quotient Rules and Higher-Order Derivatives]]

Next - [[2.5]]
# Content

## [[Chain Rule]]

This text has yet to discuss one of the most powerful differentiation rules—the **[[Chain Rule]].** This rule deals with composite functions and adds a surprising versatility to the rules discussed in the two preceding sections. For example, compare the functions shown below. Those on the left can be differentiated without [[Chain Rule]], and those on the right are best differentiated with [[Chain Rule]].

| Without [[Chain Rule]] | With [[Chain Rule]] |
| ---------------------- | ------------------- |
| $y=x^2+1$              | $y=\sqrt{ x^2+1 }$  |
| $y=\sin x$             | $y=\sin6x$          |
| $y=3x+2$               | $y=(3x+2)^5$        |
| $y=x+\tan x$           | $y=x+\tan x^2$      |

Basically, [[Chain Rule]] states that if $y$ changes $\frac{dy}{du}$ times as fast as $u$, and $u$ changes $\frac{du}{dx}$ times as fast as $x$, then $y$ changes $\left( \frac{dy}{du} \right)\left( \frac{du}{dx} \right)$ times as fast as $x$.

>[!faq] Example
>Figure 2.24 shows a set of gears. The second and third gears are on the same axle. As the first axle revolves, it drives the second axle, which in turn drives the third axle. Let __y__, __u__, and __x__ represent the numbers of revolutions per minute of the first, second, and third axles, respectively. Find $\frac{dy}{du}$, $\frac{du}{dx}$, and $\frac{dy}{dx}$, and show that $$\frac{dy}{dx}=\frac{dy}{du}*\frac{du}{dx}$$
>![[Pasted image 20240916090920.png]]
>
>Solution:
>Because the circumference of the second gear is three times that of the first, the first axle must make three revolutions to turn the second axle once. Similarly, the second axle must make two revolutions to turn the third axle once, so: $$\frac{dy}{du}=3$$
>and $$\frac{du}{dx}=2$$
>Combining these two results, note that the first axle must make six revolutions to turn the third axle once. So, you can write:
>$\frac{dy}{dx}=$Rate of change of first axle with respect to second axle * Rate of change of second axle with respect to third axle
>$$=\frac{dy}{du}*\frac{du}{dx}$$
>$$=3*2$$
>$=6=$Rate of change of first axle with respect to the third axle
>In other words, the rate of change of __y__ with respect to __x__ is the product of the rate of change of __y__ with respect to __u__ and the rate of change of __u__ with respect to __x__.

>[!info] The Chain Rule
>If $y=f(u)$ is a differentiable [[function]] of __u__ and $u=g(x)$ is a differentiable [[function]] of __x__, then $y=f(g(x))$ is a differentiable [[function]] of __x__ and:
>$$\frac{dy}{dx}=\frac{dy}{du}*\frac{du}{dx}$$
>or, equivalently: $$\frac{d}{dx}[f(g(x))]=f'(g(x))g'(x)$$
>When applying [[Chain Rule]], it is helpful to think of the composite [[function]] $f\circ g$ as having two parts—an inner part and an outer part.
>
>![[Pasted image 20240916092233.png]]

^87f17e

>[!faq] Example: Decomposition of a Composite [[Function]]
>![[Pasted image 20240916093230.png]]

>[!faq] Example: Using [[Chain Rule]]
>Find $\frac{dy}{dx}$ for: $$y=(x^2+1)^3$$
>
>Solution:
>For this [[function]], let the inside [[function]] be $u=x^2+1$ and the outer [[function]] be $y=u^3$. By [[Chain Rule]], you obtain:
>
>![[Pasted image 20240916094302.png]]
> >[!note]
> >You could also solve this problem without using [[Chain Rule]] by expanding the binomial to obtain:
> >$$y=x^6+3x^4+3x^2+1$$
> >and then finding the [[derivative]]
> >$$y'=6x^5+12x^3+6x$$
> >Verify that this is the same as the [[derivative]]. Which method would you use to find:
> >$$\frac{d}{dx}[(x^2+1)^50]$$

>[!abstract] Exploration: Using [[Chain Rule]]
>Each [[function]] below can be differentiated using rules that you studied in Sections 2.2 and 2.3. For each [[function]], find the [[derivative]] using those rules. Then find the [[derivative]] using [[Chain Rule]]. Compare your results. Which method is simpler?
>1. $y=\frac{2}{3x+1}$
>2. $y=(x+2)^3$
>3. $y=\sin 2x$

## [[General Power Rule]]

The [[function]] in Example [[Chain Rule]] is an example of one of the most common types of composite functions, $y=[u(x)]^n$. The rule for differentiating such functions is called the **[[General Power Rule]],** and it is a special case of [[Chain Rule]].

>[!note] The General Power Rule
>If $y=[u(x)]^n$, where __u__ is a differentiable [[function]] of __x__ and __n__ is a rational number, then:
>$$\frac{dy}{dx}=n[u(x)]^{n-1}\frac{du}{dx}$$
>or equivalently
>$$\frac{d}{dx}[u^n]=n u^{n-1}u'$$

^94013a

>[!faq]- Applying [[General Power Rule]]
>Find the [[derivative]] of $f(x)=(3x-2x^2)^3$
>
>Solution:
>Let $u=3x-2x^2$.
>
>Then: $$f(x)=(3x-2x^2)^3=u^3$$
>By [[General Power Rule]] the [[derivative]] is:
>![[Pasted image 20240916105842.png]]

>[!faq]- Differentiating a [[function]] involving a radical
>Find all points on the graph of: $$f(x)=^3\sqrt{ (x^2-1)^2 }$$
>for which $f'(x)=0$ and those for which $f'(x)$ does not exist.
>
>Solution:
>Begin by rewriting the [[function]] in rational exponent form:
>$$f(x)=(x^2-1)^{2/3}$$
>Then, applying [[General Power Rule]] (with $u=x^2-1$) produces:
>![[Pasted image 20240916111756.png]]
>
>So, $f(x)=0$ when $x=0$, and $f'(x)$ does not exist when $x=\pm1$ as shown here:
>![[Pasted image 20240916112018.png]]
>
>The [[derivative]] of __f__ is __0__ at $x=0$ and is undefined at $x=\pm1$

>[!faq]- Differentiating a Quotient: Constant Numerator
>Differentiate the [[function]]: $$g(t)=\frac{-7}{(2t-3)^2}$$
>
>Solution:
>Begin by rewriting the [[function]] with a negative exponent:
>$$g(t)=-7(2t-3)^2$$
>
>Then apply [[General Power Rule]] with $u=2t-3$ which produces:
>![[Pasted image 20240916114709.png]]
> >[!note]
> >Try differentiating the [[function]] in Example 6 using the Quotient Rule. You should obtain the same result, but using the Quotient Rule is less efficient than using [[General Power Rule]].

## Simplifying Derivatives

>[!faq]- Simplifying by factoring out the least power
>Find the [[derivative]] of $f(x)=x^2\sqrt{ 1-x^2 }$
>
> >[!info]- Solution
> >Rewrite: $$=x^2\sqrt{ 1-x^2 }$$
> >The Product Rule: $$=x^2\frac{d}{dx}\left[ (1-x^2)^{\frac{1}{2}} \right]+(1+x^2)^{\frac{1}{2}}\frac{d}{dx}[x^2]$$
> >[[General Power Rule]]: $$=x^2\left[ \frac{1}{2}(1-x)^{\frac{1}{2}}(-2x) \right]+(1-x^2)^{\frac{1}{2}}(2x)$$
> >Simplify: $$=-x^3(1-x^2)^{-\frac{1}{2}}+2x(1-x^2)^{\frac{1}{2}}$$
> >Factor: $$x(1-x^2)^{-\frac{1}{2}}[-x^2(1)+2(1-x^2)]$$
> >Simplify: $$x(1-x^2)^{-\frac{1}{2}}(2-3x^2)$$
> >Write in radical form: $$\frac{x(2-3x^2)}{\sqrt{ 1-x^2 }}$$
> > >[!note]
> > >You can subtract exponents when factoring. That is, when $(1-x^2)^{-\frac{1}{2}}$ is factored out of $(1-x^2)^{\frac{1}{2}}$ , the remaining factor has an exponent of $\frac{1}{2}-\left( \frac{1}{2} \right)=1$. So, $(1-x^2)^{\frac{1}{2}}$ is equal to the product of $(1-x^2)^{-\frac{1}{2}}$ and $(1-x^2)^1$.

>[!faq]- Simplifying the [[derivative]] of a quotient
>Original [[function]] $$f(x)=\frac{x}{^3\sqrt{ x^2+4 }}$$
> >[!info]- Solution
> >Rewrite: $$=\frac{x}{(x^2+4)^{\frac{1}{2}}}$$
> >Quotient Rule: $$(x^2+4)^{\frac{1}{3}}(1)-x\left( \frac{1}{3} \right)(x^2+4)^{-\frac{2}{3}}(2x)$$
> >Factor: $$=\frac{1}{3}(x^2+4)^{-\frac{2}{3}}\left[ \frac{3(x^2+4)-(2x^2)(1)}{(x^2+4)^{\frac{2}{3}}} \right]$$
> >Simplify: $$\frac{x^2+12}{3(x^2+4)^{\frac{4}{3}}}$$
> > >[!note]
> > >Some graphing utilities are capable of differentiating very complicated functions. Often, however, the result is given in unsimplified form. If you have access to such a utility, use it to find the derivatives of the functions given in Examples 7, 8, and 9. Then compare the results with those given in these examples.

>[!faq]- Simplifying the [[derivative]] of a power
>Original [[function]]: $$y=\left( \frac{3x-1}{x^+3} \right)^2$$
> >[!info]- Solution
> >[[General Power Rule]]: $$y'=2\left( \frac{3x-1}{x^2+3} \right)\frac{d}{dx}\left[ \frac{3x-1}{x^2+3} \right]$$
> >Quotient Rule: $$\left[ \frac{2(3x-1)}{x^2+3} \right]\left[ \frac{(x^2+3)(3)-(3x-1)(2x)}{(x^2+3)^2} \right]$$
> >Multiply: $$\frac{2(3x-1)(3x^2+9-6x^2+2x)}{(x^2+3)^3}$$
> >Simplify: $$=\frac{2(3x-1)(-3x^2+2x+9)}{(x^2+3)^3}$$

## Trigonometric Functions and [[Chain Rule]]

The “[[Chain Rule]] versions” of the derivatives of the six trigonometric functions are shown below.

![[Pasted image 20240916131423.png]]

>[!faq]- The [[chain rule]] and trigonometric functions
>![[Pasted image 20240916131721.png]]

>[!faq]- Parenthesis and trigonometric functions
>![[Pasted image 20240916132059.png]]
> >[!note]
> >Another way to write the [[derivative]] in Example 11(d) is to use the double angle identity, $2\sin x\cos x=\sin 2x$. Applying this identity, the result is:
> >$$y'=-2\cos x\sin x$$
> >$$=-(2\sin x\cos x)$$
> >$$=-\sin2x$$

>[!faq]- Repeated application of the [[chain rule]]
>Original [[function]]: $f(t)=\sin^34t$
> >[!info]- Solution
> >Rewrite: $$=(\sin 4t)^3$$
> >Apply [[chain rule]] once: $$f'(t)=3(\sin 4t)^2\frac{d}{dt}[\sin 4t]$$
> >Apply [[chain rule]] again: $$3(\sin 4t)^2(\cos 4t)\frac{d}{dt}[4t]$$
> >$$3(\sin 4t)^2(\cos 4t)(4)$$
> >Simplify: $$12\sin^24t\cos 4t$$

>[!faq]- Tangent Line of a trigonometric [[function]]
>Find an equation of the tangent line of the graph of $f(x)=2\sin+\cos 2x$ at the point $(\pi,1)$ as shown below. Then determine all values of __x__ in the interval $(0,2\pi)$ at which the graph of __f__ has a horizontal tangent.
>![[Pasted image 20240916134125.png]]
> >[!info]- Solution
> >Begin by finding $f'(x)$: $$f(x)=2\sin+\cos 2x$$
> >Apply [[chain rule]] to $\cos 2x$: $$f'(x)=2\cos x+(-\sin 2x)(2)$$
> >Simplify: $$=2\cos x-2\sin 2x$$
> >To find the slope of the tangent line at $(\pi,1)$, evaluate $f'(\pi)$
> >Substitute: $$f'(\pi)=2\cos \pi-2\sin 2\pi$$
> >Slope of the tangent line at $(\pi,1)$: $$=-2$$
> >Now, use the point-slope form of the equation of a line to write.
> >Point-slope form: $$y-y_{1}=m(x-x_{1})$$
> >Substitute for $y_{1},m,x_{1}$: $$y-1=-2(x-\pi)$$
> >Equation of the tangent line at $(\pi,1)$: $$y=-2x+1+2\pi$$
> > >[!note]
> > >$f'(x)=0$ in the interval $(0,2\pi)$ when $x=\frac{\pi}{6},\frac{\pi}{2},\frac{5\pi}{6},\frac{3\pi}{2}$. So, the graph of __f__ has horizontal tangents at $x=\frac{\pi}{6},\frac{\pi}{2},\frac{5\pi}{6},\frac{3\pi}{2}$

This section concludes with a summary of the differentiation rules studied so far. To become skilled at differentiation, you should learn each rule in words, not symbols. As an aid to memorization, note that the cofunctions (cosine, cotangent, and cosecant) require a negative sign as part of their derivatives.

>[!note] Summary of Differentiation Rules
>![[Pasted image 20240916135644.png]]

# References
