# Summary
# Related
Prev - [[P.5 Factoring with Negative and Rational Exponents]]
Next - [[1.3 Graphing]]
# Content

>[!info] Types of Partial Fractions
>1. Denominator - Unique linear factor
>2. Denominator - Repeated linear factor
>3. Denominator - Unique quadratic factor

>[!faq]- $\frac{9x+21}{x^2+2x-15}$
>We want unique linear factors, so find the factors of the denominator first.
>$\frac{9x+21}{(x+5)(x-3)}$
>The numerator is a __constant__ in _linear factors_
>$\frac{A}{x+5}+\frac{B}{x-3}$ Made different letters because they are also _unique_
>$$(x+5)(x-3)\left( \frac{A}{x+5} \right)+(x+5)(x-3)\left( \frac{B}{x-3} \right)$$
>Cancel out like terms
>$$9x+21=A(x-3)+B(x+5)$$
>Now just solve, first distribute
>$9x+21=Ax-3A+Bx+5B$
>Like terms again, they're not really like terms but the __A__ and __B__ aren't really numbers so they can be considered such.
>$$9x+21=(Ax+Bx)+(-3A+5B)$$
>$9x+21=(A+B)x+(-3A+5B)$
>Equate the coefficients of like terms
>$9=A+B$ 
>$21=-3A+5B$ Constant terms
>Now solve using the Substitution Method
>$9=A+B$ For A
>$A=9-B$
>Put that in the second equation
>$21=-3(9-B)+5B$
>Solve for __B__
>$21=-27+3B+5B$
>$48=8B$
>$B=6$
>Plug it back in to $A=9-B$
>$A=9-6$
>$A=3$
>Finally, plug it back into the original
>$\frac{3}{x+5}+\frac{6}{x-3}$

>[!faq]- Repeating linear factor $\frac{x}{(x-1)^2}$
>Common factor
>$=\frac{A}{x-1}+\frac{B}{(x-1)^2}$
>$$(x-1)^2\left( \frac{x}{(x-1)^2} \right)=(x-1)^2\left( \frac{A}{x-1} \right)+(x-1)^2\left( \frac{B}{(x-1)^2} \right)$$
>Like terms
>$x=A(x-1)+B$
>Distribute
>$x=Ax-A+B$
>Now solve
>$x=Ax \to A=1$
>$-A+B=0\to -1+B=0\to B=1$

>[!faq]- Quadratic Factor $\frac{9x-2}{(x-2)(x^2+2x+3)}$
>Each numerator will be different, but the second will be quadratic
>$$\frac{9x-2}{(x-2)(x^2+2x+3)}=\frac{A}{x-2}+\frac{Bx+C}{x^2+2x+3}$$
>Now set it up
>$$(x-2)(x^2+2x+3)\left( \frac{9x-2}{(x-2)(x^2+2x+3)} \right)=(x-2)(x^2+2x+3)\left( \frac{A}{x-2} \right)+(x-2)(x^2+2x+3)\left( \frac{Bx+C}{x^2+2x+3} \right)$$
>Cancel out like terms
>$$9x-2=A(x^2+2x+3)+(x-2)(Bx+C)$$
>Distribute and foil
>$$9x-2=Ax^2+2Ax+3A+Bx^2+Cx-2Bx-2C$$
>Group the similar terms, taking out the common
>$$9x-2=(A+B)x^2+(2A+C-2B)x+(3A-2C)$$
>Solve
>	Equation 1: $A+B=0$
>	Equation 2: $2A-2B+C=9$
>	Equation 3: $3A-2C=-2$
>__Note:__ _This is an identity from Trigonometry that has infinite solutions_ $0=0$

>[!faq]- $\frac{10x^2+2x}{(x-1)(x^2+2)}$
>Denominators
>$$=\frac{A}{x-1}+\frac{Bx+C}{x^2+2}$$
>Set it up
>$$((x-1)(x^2+2))\left( \frac{10x^2+2x}{(x-1)(x^2+2)} \right)=(x-1)(x^2+2)\left( \frac{A}{x-1} \right)+(x-1)(x^2+2)\left( \frac{Bx+C}{x^2+2} \right)$$
>Cancel out like terms
>$$10x^2+2x=(x^2+2)(A)+(x-1)(Bx+C)$$
>Distribute and foil
>$$10x^2+2x=(A+B)x^2+(-B+C)x+(2A-C)$$
>Find your equations
>	Equation 1: $A+B=10$
>	Equation 2: $-B+C=2$
>	Equation 3: $2A-C=0$
>First, try adding the first two equations to do __Elimination__
>$$(A+B=10)+(-B+C=2)\to A+C=12$$
>Then solve the rest
>$2A-C=0$
>$3A=12$
>$A=4$
>$4+b=10$
>$B=6$
>$-6+C=2$
>$C=8$

# References